base case for estimate complete.

src/Protocol.v
@@ -1,6 +1,7 @@
 Require Import Blocks.
 Require Import Votes.
 Require Import Preliminars.
+Require Import List.
 
 
 Definition Time := nat.
@@ -11,18 +12,20 @@ Inductive RoundState
   (precommit_voters: Voters precommit_number)
   (round_start_time:Time) 
   (last_block: Block last_block_number)
-    : Time ->  Type :=
+  : nat -> Time ->  Type :=
   | InitialRoundState 
-    : RoundState preview_voters precommit_voters round_start_time last_block 0
+    : RoundState preview_voters precommit_voters round_start_time last_block 0 0
   | RoundStateUpdate 
+    {round_number}
     {old_time_increment: Time}
     (old_state: RoundState 
       preview_voters precommit_voters 
-      round_start_time last_block old_time_increment)
+      round_start_time last_block round_number old_time_increment)
     (time_increment: Time)
     (new_preview_votes: Votes preview_voters last_block)
     (new_precommit_votes: Votes precommit_voters last_block)
     : RoundState preview_voters precommit_voters round_start_time last_block 
+      round_number
       (time_increment+ old_time_increment).
 
 Section State1.
@@ -33,22 +36,23 @@ Context {precommit_voters: Voters precommit_number}.
 Context {last_block: Block last_block_number}.
 Context {round_time : Time}.
 Context {round_number: nat}.
+Context {time_increment: nat}.
 
 
 
 
 Definition get_preview_votes
-  (round_state: RoundState preview_voters precommit_voters  round_time last_block round_number)
+  (round_state: RoundState preview_voters precommit_voters  round_time last_block round_number time_increment)
   : 
   (Votes preview_voters last_block)
   := 
   match round_state with
-  | InitialRoundState _ _ _ _ => VotesC _ _ List.nil (* No votes in initial round state *)
+  | InitialRoundState _ _ _ _ => VotesC _ _ List.nil 
   | RoundStateUpdate _ _ _ _ _ _ new_preview_votes _ => new_preview_votes
   end.
 
 Definition get_precommit_votes
-  (round_state: RoundState preview_voters precommit_voters  round_time last_block round_number)
+  (round_state: RoundState preview_voters precommit_voters  round_time last_block round_number time_increment)
   : 
   (Votes precommit_voters last_block)
   :=
@@ -59,6 +63,42 @@ Definition get_precommit_votes
 
 End State1.
 
+Fixpoint get_all_preview_votes{preview_number precommit_number : nat}
+  {preview_voters : Voters preview_number} 
+  {precommit_voters: Voters precommit_number}
+  {round_time:Time}
+  {round_number:nat}
+  {last_block_number} 
+  {last_block : Block last_block_number} 
+  {time_increment: Time}
+  (round_state: RoundState preview_voters precommit_voters  round_time last_block round_number time_increment)
+  : 
+  (Votes preview_voters last_block)
+  := 
+  match round_state with
+  | InitialRoundState _ _ _ _ => VotesC _ _ List.nil 
+  | RoundStateUpdate _ _ _ _ old_state  _ new_preview_votes _ => mergeVotes (get_all_preview_votes old_state) new_preview_votes
+  end.
+
+Fixpoint get_all_precommit_votes{preview_number precommit_number : nat}
+  {preview_voters : Voters preview_number} 
+  {precommit_voters: Voters precommit_number}
+  {round_time:Time}
+  {round_number:nat}
+  {last_block_number} 
+  {last_block : Block last_block_number} 
+  {time_increment: Time}
+  (round_state: RoundState preview_voters precommit_voters  round_time last_block round_number time_increment)
+  : 
+  (Votes precommit_voters last_block)
+  := 
+  match round_state with
+  | InitialRoundState _ _ _ _ => VotesC _ _ List.nil 
+  | RoundStateUpdate _ _ _ _ old_state  _ _ new_precommit_votes => mergeVotes (get_all_precommit_votes old_state) new_precommit_votes
+  end.
+
+
+
 Variant Estimate {preview_number precommit_number : nat}
   {preview_voters : Voters preview_number} 
   {precommit_voters: Voters precommit_number}
@@ -66,7 +106,8 @@ Variant Estimate {preview_number precommit_number : nat}
   {round_number:nat}
   {last_block_number} 
   {last_block : Block last_block_number} 
-  (round_state: RoundState preview_voters precommit_voters  round_time last_block round_number)
+  {time_increment: Time}
+  (round_state: RoundState preview_voters precommit_voters  round_time last_block round_number time_increment)
   : {n & Block n} -> Type
   :=
     | EstimateOrigin : round_number = 0 -> Estimate round_state (existT _ 0 OriginBlock)
@@ -90,10 +131,11 @@ Context {precommit_voters: Voters precommit_number}.
 Context {last_block: Block last_block_number}.
 Context {round_time : Time}.
 Context {round_number: nat}.
+Context {time_increment : Time}.
 
 
 Definition get_estimate_block
-  {round_state: RoundState preview_voters precommit_voters  round_time last_block round_number}
+  {round_state: RoundState preview_voters precommit_voters  round_time last_block round_number time_increment}
   {n}
   {block : Block n}
   (estimate :Estimate round_state (existT _ n block))
@@ -104,32 +146,8 @@ Definition get_estimate_block
     | EstimateC _ new_block _ _ _ _ => new_block
   end.
 
-Print get_preview_votes.
 
-Definition get_round_number
-  (round_number2:Time)
-  (round_state: RoundState preview_voters precommit_voters  round_time last_block round_number2)
-  : Type
-  :=
-    match round_state with 
-    | InitialRoundState _ _ _ _ => RoundState preview_voters precommit_voters round_time last_block 0
-    | _ => RoundState preview_voters precommit_voters round_time last_block round_number2
-    end.
-
-Definition get_estimate_case_1
-  (round_state: RoundState preview_voters precommit_voters  round_time last_block 0)
-  : option (Estimate round_state (existT _ 0 OriginBlock))
-  :=
-    match round_state with 
-    | InitialRoundState _ _ _ _ => Some (EstimateOrigin round_state eq_refl)
-    | _ => None
-    end.
-
-Require Import Equality.
-Print block.
-Locate block.
-
-Definition get_estimate (round_state: RoundState preview_voters precommit_voters  round_time last_block round_number)
+Definition get_estimate (round_state: RoundState preview_voters precommit_voters  round_time last_block round_number time_increment)
   : option {n & { block & Estimate round_state (existT _ n block)}}
   :=
  match round_state  with
@@ -146,47 +164,28 @@ Definition get_estimate (round_state: RoundState preview_voters precommit_voters
           )
         )
       )
-  | _ => None
-  end.
-
-Definition get_estimate 
-  (round_state: RoundState preview_voters precommit_voters  round_time last_block round_number)
-  : option {n & { block & Estimate round_state (existT _ n block)}}.
-Proof.
-  dependent destruction  round_state.
-  - refine (Some (existT _ 0 (existT _ OriginBlock (EstimateOrigin (InitialRoundState preview_voters precommit_voters round_time last_block) eq_refl))) ).
-  - refine None.
-Qed.
-
-
-Print get_estimate.
-  :=
- match round_state in RoundState _ _ _ _ 0 return option {n & { block & Estimate round_state (existT _ n block)}} with
-  | InitialRoundState _ _ _ _ =>None
-      (*Some (existT _ 0 (existT _ OriginBlock (EstimateOrigin round_state _)))*)
-  | b => False_rect unit
-  end.
-  match round_number with
-  | O =>
-    Some (existT _ 0 (existT _ _ OriginBlock, EstimateOrigin eq_refl))
-  | _ => g preview_votes
-
+  | RoundStateUpdate _ _ _ _ _ _ _ _=> 
+    let all_preview_votes := get_all_preview_votes round_state
+    in
+    let all_precommit_votes := get_all_precommit_votes round_state
+    in
+    None
   end.
 
 
 Variant Completable 
-  (round_state: RoundState preview_voters precommit_voters  round_time last_block round_number)
+  (round_state: RoundState preview_voters precommit_voters  round_time last_block round_number time_increment)
   : Type
   :=
-  | CompletableBelowPreview {estimate_block_number}
-      (e: Estimate  round_state estimate_block_number)
+  | CompletableBelowPreview {number_and_block}
+      (e: Estimate  round_state number_and_block)
       {g_block_number: nat}
       (g_preview: Block g_block_number)
       (g_preview_is_some 
         : g ( get_preview_votes round_state) 
           = Some (existT _ g_block_number g_preview)
       )
-      (new_block_is_below_g: estimate_block_number < g_block_number)
+      (new_block_is_below_g: projT1 number_and_block < g_block_number)
   | CompletableByImpossible 
       {g_block_number: nat}
       (g_preview: Block g_block_number)
